\textcolor{blue}{Problem 4}

4.33 Chain inequality. Let $X_1 \rightarrow X_2 \rightarrow X_3 \rightarrow X_4$ form a Markov chain. Show that
    $$I\left(X_1 ; X_3\right)+I\left(X_2 ; X_4\right) \leq I\left(X_1 ; X_4\right)+I\left(X_2 ; X_3\right)$$

\textcolor{blue}{Solution}

From the chain rule of mutual information, we have
\begin{align*}
I\left(X_1,X_2;X_3\right) &= I\left(X_1;X_3\right) + I\left(X_2;X_3|X_1\right) \\
&= I\left(X_2;X_3\right) + I\left(X_1;X_3|X_2\right) \\
I\left(X_1,X_2;X_4\right) &= I\left(X_1;X_4\right) + I\left(X_2;X_4|X_1\right) \\
&= I\left(X_2;X_4\right) + I\left(X_1;X_4|X_2\right) \\
I\left(X_3,X_4;X_2|X_1\right) &= I\left(X_3;X_2|X_1\right) + I\left(X_4;X_2|X_1,X_3\right) \\
&= I\left(X_4;X_2|X_1\right) + I\left(X_3;X_2|X_1,X_4\right)
\end{align*}

From the property of Markov chain, we have
\begin{align*}
I\left(X_1;X_3|X_2\right) &= 0 \\
I\left(X_1;X_4|X_2\right) &= 0 \\
I\left(X_2;X_4|X_1,X_3\right) &= 0
\end{align*}

So we have
\begin{equation}
I\left(X_1;X_3\right) - I\left(X_2;X_3\right) = -I\left(X_2;X_3|X_1\right)
\label{eq:1}
\end{equation}
\begin{equation}
I\left(X_2;X_4\right) - I\left(X_1;X_4\right) = I\left(X_2;X_4|X_1\right)
\label{eq:2}
\end{equation}
\begin{equation}
I\left(X_3;X_2|X_1\right) - I\left(X_4;X_2|X_1\right) = I\left(X_2;X_3|X_1,X_4\right)
\label{eq:3}
\end{equation}

So we have
\begin{align*}
&\ \ \ \ I\left(X_1;X_3\right) + I\left(X_2;X_4\right) - I\left(X_1;X_4\right) - I\left(X_2;X_3\right) \\
&= \left[I\left(X_1;X_3\right) - I\left(X_2;X_3\right) \right] + \left[I\left(X_2;X_4\right) - I\left(X_1;X_4\right)\right] \\
&= I\left(X_2;X_4|X_1\right) - I\left(X_2;X_3|X_1\right) \text{\ \ \ \ \ \ \ \ \ \ (from (\ref{eq:1}) and (\ref{eq:2}))} \\
&= -I\left(X_2;X_3|X_1,X_4\right) \text{\ \ \ \ \ \ \ \ \ \ \ \ \ \ \ \ \ \ \ \ \ \ \ \ (from (\ref{eq:3}))} \\
&\leq 0 \text{\ \ \ \ \ \ \ \ \ \ \ \ \ \ \ \ \ \ \ \ \ \ \ \ \ \ \ \ \ \ \ \ \ \ \ \  \ \ \ \ \ \ \ \ \ \ \ \ (property of mutual information)}
\end{align*}

So above all, we have proved that
$$I\left(X_1 ; X_3\right)+I\left(X_2 ; X_4\right) \leq I\left(X_1 ; X_4\right)+I\left(X_2 ; X_3\right)$$

\newpage